theories/Bigstep.v
@@ -12,6 +12,12 @@ Inductive eval_expr : heap -> var_set -> expr ->
       whnf w ->
       eval_expr G L w G w
 
+  | EvalBop : forall G L op e1 e2 n1 n2 n D1 D2,
+      eval_expr G L e1 D1 (ENat n1) ->
+      eval_expr D1 L e2 D2 (ENat n2) ->
+      eval_bop op n1 n2 = Some n ->
+      eval_expr G L (EBop op e1 e2) D2 (ENat n)
+
   | EvalSat : forall G L m e D O w,
       matching_arity m = Some 0 ->
       eval_matching G L [] m D (MRReturn e) ->
@@ -48,6 +54,11 @@ with eval_matching : heap -> var_set -> list var -> matching ->
   | EvalBindVar : forall G L A x y m D u,
       eval_matching G L A (subst_matching m y x) D u ->
       eval_matching G L (y :: A) (MMatch (PVar x) m) D u
+
+  | EvalNatMatch : forall G L A x n m D u,
+      eval_expr G L (EVar x) G (ENat n) ->
+      eval_matching G L A m D u ->
+      eval_matching G L (x :: A) (MMatch (PNat n) m) D u
 
   | EvalConsMatch : forall G L A x cp ps m args D O u,
       eval_expr G L (EVar x) D (ECons cp (map EVar args)) ->
@@ -89,7 +100,7 @@ Combined Scheme eval_ind from eval_expr_ind_mutual, eval_matching_ind_mutual.
 Lemma eval_expr_produces_whnf : forall G L e D w,
   eval_expr G L e D w -> whnf w.
 Proof.
-  intros. induction H; assumption.
+  intros. induction H; try assumption; try constructor.
 Qed.
 
 (* Determinism *)
@@ -140,9 +151,24 @@ Proof.
   - intros G L e D1 w1 D2 w2 H1 H2.
     induction H1; inversion H2; subst; try congruence.
     + auto.
+    + inversion H.
     + inversion H; subst. rewrite H0 in H5. discriminate.
     + inversion H.
     + inversion H.
+    + inversion H0.
+    + assert (H_e1: D1 = D3 /\ ENat n1 = ENat n0).
+      { solve_determinism_expr eval_expr_deterministic; auto. }
+      destruct H_e1 as [HeqD1 Heqw1].
+      injection Heqw1 as Heqn1; subst D3 n0.
+
+      assert (H_e2: D0 = D2 /\ ENat n2 = ENat n3).
+      { eapply eval_expr_deterministic; eauto. }
+      destruct H_e2 as [HeqD2 Heqw2].
+      injection Heqw2 as Heqn2; subst D2 n3.
+
+      rewrite H in H10.
+      injection H10 as Heq; subst n4.
+      auto.
     + inversion H3. subst. rewrite H5 in H. discriminate.
     + solve_determinism_match eval_matching_deterministic.
       inversion Hequ; subst.
